Cleanup: move generic defs to project-everest/everparse@eeb73d7c56f9c2553c915a8dc45c9274a05021f5

src/tls/ParsersAux.Binders.Aux.fst
@@ -20,8 +20,6 @@ friend Parsers.ClientHelloExtensions
 friend Parsers.ClientHello
 friend Parsers.Handshake_m_client_hello
 
-open ParsersAux.Seq
-
 let serialize_offeredPsks_eq
   o
 = LP.serialize_synth_eq _ Psks.synth_offeredPsks Psks.offeredPsks'_serializer Psks.synth_offeredPsks_recip () o;
@@ -42,46 +40,9 @@ let serialize_list_clientHelloExtension_eq
   LP.serialize_list_append _ CHE.clientHelloExtension_serializer (L.init l) [L.last l];
   LP.serialize_list_singleton _ CHE.clientHelloExtension_serializer (L.last l)
 
-#push-options "--z3rlimit 16"
-
-let rec serialize_list_eq_parser_fail
-  (#k: LP.parser_kind)
-  (#t: Type)
-  (#p: LP.parser k t)
-  (s: LP.serializer p { k.LP.parser_kind_subkind == Some LP.ParserStrong /\ k.LP.parser_kind_low > 0 })
-  (l1 l2: list t)
-  (b1 b2: LP.bytes)
-: Lemma
-  (requires (
-    LP.serialize (LP.serialize_list _ s) l1 `Seq.append` b1 == LP.serialize (LP.serialize_list _ s) l2 `Seq.append` b2 /\
-    LP.parse p b1 == None /\
-    LP.parse p b2 == None
-  ))
-  (ensures (l1 == l2 /\ b1 == b2))
-  (decreases (L.length l1))
-= LP.serialize_list_nil _ s;
-  assert (b1 `Seq.equal` (Seq.append Seq.empty b1));
-  assert (b2 `Seq.equal` (Seq.append Seq.empty b2));
-  if L.length l2 < L.length l1
-  then serialize_list_eq_parser_fail s l2 l1 b2 b1
-  else match l1, l2 with
-  | [], [] -> ()
-  | x1 :: l1', x2 :: l2' ->
-    LP.serialize_list_cons _ s x1 l1' ;
-    LP.serialize_list_cons _ s x2 l2' ;
-    Seq.append_assoc (LP.serialize s x1) (LP.serialize (LP.serialize_list _ s) l1') b1;
-    Seq.append_assoc (LP.serialize s x2) (LP.serialize (LP.serialize_list _ s) l2') b2;
-    LP.serialize_strong_prefix s x1 x2 (LP.serialize (LP.serialize_list _ s) l1' `Seq.append` b1) (LP.serialize (LP.serialize_list _ s) l2' `Seq.append` b2);
-    serialize_list_eq_parser_fail s l1' l2' b1 b2
-  | [], x2 :: l2' ->
-    LP.serialize_list_cons _ s x2 l2' ;
-    LP.parse_strong_prefix p (LP.serialize s x2) b1
-
-#pop-options
-
 let serialize_list_clientHelloExtension_inj_prefix
   l1 l2 b1 b2
-= serialize_list_eq_parser_fail CHE.clientHelloExtension_serializer l1 l2 b1 b2
+= LP.serialize_list_eq_parser_fail CHE.clientHelloExtension_serializer l1 l2 b1 b2
 
 let size32_list_clientHelloExtension
   l
@@ -91,95 +52,9 @@ module HST = FStar.HyperStack.ST
 module B = LowStar.Buffer
 module HS = FStar.HyperStack
 
-#push-options "--z3rlimit 16"
-
-inline_for_extraction
-let rec list_last_pos
-  (#k: _)
-  (#t: _)
-  (#p: LP.parser k t)
-  (s: LP.serializer p)
-  (j: LP.jumper p)
-  (#rrel #rel: _)
-  (sl: LP.slice rrel rel)
-  (pos pos' : U32.t)
-  (l: Ghost.erased (list t))
-: HST.Stack U32.t
-  (requires (fun h ->
-    k.LP.parser_kind_subkind == Some LP.ParserStrong /\
-    k.LP.parser_kind_low > 0 /\
-    LP.live_slice h sl /\
-    U32.v pos <= U32.v pos' /\
-    U32.v pos' <= U32.v sl.LP.len /\
-    LP.bytes_of_slice_from_to h sl pos pos' `Seq.equal` LP.serialize (LP.serialize_list _ s) (Ghost.reveal l) /\
-    Cons? (Ghost.reveal l)
-  ))
-  (ensures (fun h res h' ->
-    B.modifies B.loc_none h h' /\
-    U32.v pos + Seq.length (LP.serialize (LP.serialize_list _ s) (L.init (Ghost.reveal l))) == U32.v res
-  ))
-= let h0 = HST.get () in
-  HST.push_frame ();
-  let h1 = HST.get () in
-  let bgleft = B.alloca (Ghost.hide ([] <: list t)) 1ul in
-  let bgright = B.alloca l 1ul in
-  let bpos1 = B.alloca pos 1ul in
-  LP.serialize_list_nil _ s;
-  let _ = C.Loops.do_while
-    (fun h stop ->
-      B.modifies (B.loc_region_only true (HS.get_tip h1)) h1 h /\
-      B.live h bgleft /\
-      B.live h bgright /\
-      B.live h bpos1 /\ (
-      let left = Ghost.reveal (Seq.index (B.as_seq h bgleft) 0) in
-      let right = Ghost.reveal (Seq.index (B.as_seq h bgright) 0) in
-      let pos1 = Seq.index (B.as_seq h bpos1) 0 in
-      Ghost.reveal l == left `L.append` right /\
-      U32.v pos + Seq.length (LP.serialize (LP.serialize_list _ s) left) == U32.v pos1 /\
-      U32.v pos1 <= U32.v pos' /\
-      LP.bytes_of_slice_from_to h0 sl pos1 pos' `Seq.equal` LP.serialize (LP.serialize_list _ s) right /\
-      Cons? right /\
-      (stop == true ==> L.length right == 1)
-    ))
-    (fun _ ->
-      let pos1 = B.index bpos1 0ul in
-      let gright = B.index bgright 0ul in
-      LP.serialize_list_cons _ s (L.hd (Ghost.reveal gright)) (L.tl (Ghost.reveal gright));
-      assert (LP.bytes_of_slice_from h0 sl pos1 `seq_starts_with` LP.bytes_of_slice_from_to h0 sl pos1 pos');
-      let pos2 = jump_serializer s j sl pos1 (Ghost.hide (L.hd (Ghost.reveal gright))) in
-      if pos2 = pos'
-      then begin
-        let f () : Lemma
-          (Nil? (L.tl (Ghost.reveal gright)))
-        = match L.tl (Ghost.reveal gright) with
-          | [] -> ()
-          | a :: q -> LP.serialize_list_cons _ s a q   
-        in
-        f ();
-        true
-      end else begin
-        let gleft = B.index bgleft 0ul in
-        B.upd bgleft 0ul (Ghost.hide (Ghost.reveal gleft `L.append` [L.hd (Ghost.reveal gright)]));
-        B.upd bgright 0ul (Ghost.hide (L.tl (Ghost.reveal gright)));
-        B.upd bpos1 0ul pos2;
-        L.append_assoc (Ghost.reveal gleft) [L.hd (Ghost.reveal gright)] (L.tl (Ghost.reveal gright));
-        LP.serialize_list_singleton _ s (L.hd (Ghost.reveal gright));
-        LP.serialize_list_append _ s (Ghost.reveal gleft) [L.hd (Ghost.reveal gright)];
-        false
-      end
-    )
-  in
-  let res = B.index bpos1 0ul in
-  let h = HST.get () in
-  L.init_last_def (Ghost.reveal (Seq.index (B.as_seq h bgleft) 0)) (L.hd (Ghost.reveal (Seq.index (B.as_seq h bgright) 0)));
-  HST.pop_frame ();
-  res
-
-#pop-options
-
 let list_clientHelloExtension_last_pos
   #rrel #rel sl pos pos' gl
-= list_last_pos CHE.clientHelloExtension_serializer CHE.clientHelloExtension_jumper sl pos pos' gl
+= LP.list_last_pos CHE.clientHelloExtension_serializer CHE.clientHelloExtension_jumper sl pos pos' gl
 
 let clientHelloExtensions_list_bytesize_eq'
   l
